#### Questions
##### 1. Use suitable identities to find the following products:
##### 2. Evaluate the following products without multiplying directly:
###### (i) 103 × 107 
###### Solution:
* Using (x + a)(x + b) = x<sup>2</sup> + x(a + b) + ab
* 103 × 107 can be written as (100 + 3)(100 + 7) 
* = 100<sup>2</sup> + 100 × (3 + 7) + (3×7) 
* = 10000 + 1000 + 21 
* = 11021
##### (ii) 95 × 96 
* Using (x + a)(x + b) = x<sup>2</sup> + x(a + b) + ab
* 95 × 96 can be written as (90 + 5)(90 + 6) 
* = 90<sup>2</sup> + 90 × (5 + 6) + (5×6) 
* = 8100 + 990 + 30 
* = 9120
##### (iii) 104 × 96
* Using (a + b)(a - b) = a<sup>2</sup> - b<sup>2</sup>
* 104 × 96 can be written as (100 + 4)(100 - 4) 
* = 100<sup>2</sup> - 4<sup>2</sup>
* = 10000 - 16 
* = 9984
##### 5. Factorize (i) 4x<sup>2</sup> + 9y<sup>2</sup> + 16z<sup>2</sup> + 12xy – 24yz – 16xz
* Using (x + y + z)^2 = x^2 + y^2 + z^2 + 2xy + 2yz + 2zx
* (2x + 3y - 4z)^2 = 4x^2 + 9y^2 + 16z^2 + 12xy - 24yz - 16xz

##### 7. Evaluate the following using suitable identities: (i) (99)<sup>3</sup> (ii) (102)<sup>3</sup> (iii) (998)<sup>3</sup>
###### (i) (99)<sup>3</sup>
* (99)<sup>3</sup> can be written as (100 - 1)<sup>3</sup> and expanded using (x - y)<sup>3</sup> = x<sup>3</sup> - y<sup>3</sup> - 3xy(x - y)
* = 100<sup>3</sup> - 1<sup>3</sup> - 3(100)(1)(100 - 1)
* = 1000000 - 1 -300(100 - 1) 
* = 1000000 - 1 -30000 + 300
* = 1000000 - 30301
* = 970299
###### (ii) (102)<sup>3</sup>
* (102)<sup>3</sup> can be written as (100 + 2)<sup>3</sup> and expanded using (x + y)<sup>3</sup> = x<sup>3</sup> + y<sup>3</sup> + 3xy(x + y)
###### (iii) (998)<sup>3</sup>
* (998)<sup>3</sup> can be written as (1000 - 2)<sup>3</sup> and expanded using (x - y)<sup>3</sup> = x<sup>3</sup> - y<sup>3</sup> - 3xy(x - y)
##### 9. Verify : (i) x<sup>3</sup> + y<sup>3</sup> = (x + y) (x <sup>2</sup> – xy + y <sup>2</sup>) 
###### Solution:
RHS = (x + y) (x<sup>2</sup> – xy + y<sup>2</sup>) <br> 
= x(x<sup>2</sup> – xy + y <sup>2</sup>) + y(x<sup>2</sup> – xy + y<sup>2</sup>) <br>
= (x<sup>3</sup> – x<sup>2</sup>y + xy<sup>2</sup>) + (yx<sup>2</sup> – xy<sup>2</sup> + y<sup>3</sup>) <br>
= x<sup>3</sup> – x<sup>2</sup>y + xy<sup>2</sup> + yx<sup>2</sup> – xy<sup>2</sup> + y<sup>3</sup> <br>
= x<sup>3</sup> + y<sup>3</sup> <br>
= LHS
##### 9. Verify : (ii) x<sup>3</sup> – y<sup>3</sup> = (x – y) (x <sup>2</sup> + xy + y <sup>2</sup>)
###### Solution:
RHS = (x - y) (x<sup>2</sup> + xy + y<sup>2</sup>) <br> 
= x(x<sup>2</sup> + xy + y <sup>2</sup>) - y(x<sup>2</sup> + xy + y<sup>2</sup>) <br>
= (x<sup>3</sup> + x<sup>2</sup>y + xy<sup>2</sup>) - (yx<sup>2</sup> + xy<sup>2</sup> + y<sup>3</sup>) <br>
= x<sup>3</sup> + x<sup>2</sup>y + xy<sup>2</sup> - yx<sup>2</sup> - xy<sup>2</sup> - y<sup>3</sup> <br>
= x<sup>3</sup> - y<sup>3</sup> <br>
= LHS
